 \documentclass[11pt]{report}

\usepackage[T2A]{fontenc}

\usepackage[utf8]{inputenc}

\usepackage[russian]{babel}

\usepackage{amsmath,amssymb}

\usepackage{graphicx}

\usepackage{caption}

\graphicspath{ {d:/HSE/Python2020/Calc/Ind8pict/} }

\oddsidemargin=-19mm

\topmargin=-30mm

\textheight 26cm 

\hsize 18cm

\textwidth 20cm

\begin{document}

\pagestyle{empty}

{\bf Индивидуальное задание.}

 
Найти асимптоты функции, заданной параметрически, изобразить на графике функцию и ее асимптоты разными цветами.

Вариант 1

$x = \sqrt{2 t + 3}$

$y = 5 + 7 / t$

Вариант 2

$x = 3 e^{t} + 3 e^{- t}$

$y = 6 e^{t} - 6 e^{- t}$

Вариант 3

$x = \frac{5 t}{t^{3} + 8}$

$y = \frac{7 t^{2}}{t^{3} + 8}$

Вариант 4

$x = \sqrt{4 t + 6}$

$y = 2 + 3 / t$

Вариант 5

$x = e^{t} + e^{- t}$

$y = 4 e^{t} - 4 e^{- t}$

Вариант 6

$x = \frac{7 t}{t^{3} + 27}$

$y = \frac{5 t^{2}}{t^{3} + 27}$

Вариант 7

$x = \sqrt{5 t + 1}$

$y = 5 + 4 / t$

Вариант 8

$x = 2 e^{t} + 2 e^{- t}$

$y = 2 e^{t} - 2 e^{- t}$

Вариант 9

$x = \frac{6 t}{t^{3} + 8}$

$y = \frac{3 t^{2}}{t^{3} + 8}$

Вариант 10

$x = \sqrt{t + 3}$

$y = 3 + 7 / t$

Вариант 11

$x = 7 e^{t} + 7 e^{- t}$

$y = 2 e^{t} - 2 e^{- t}$

Вариант 12

$x = \frac{7 t}{t^{3} + 27}$

$y = \frac{2 t^{2}}{t^{3} + 27}$

Вариант 13

$x = \sqrt{2 t + 3}$

$y = 1 + 6 / t$

Вариант 14

$x = 6 e^{t} + 6 e^{- t}$

$y = 2 e^{t} - 2 e^{- t}$

Вариант 15

$x = \frac{6 t}{t^{3} + 27}$

$y = \frac{2 t^{2}}{t^{3} + 27}$

Вариант 16

$x = \sqrt{6 t + 1}$

$y = 7 + 1 / t$

Вариант 17

$x = 2 e^{t} + 2 e^{- t}$

$y = 2 e^{t} - 2 e^{- t}$

Вариант 18

$x = \frac{4 t}{t^{3} + 27}$

$y = \frac{3 t^{2}}{t^{3} + 27}$

Вариант 19

$x = \sqrt{2 t + 3}$

$y = 5 + 7 / t$

Вариант 20

$x = 7 e^{t} + 7 e^{- t}$

$y = 5 e^{t} - 5 e^{- t}$

Вариант 21

$x = \frac{t}{t^{3} + 8}$

$y = \frac{7 t^{2}}{t^{3} + 8}$

Вариант 22

$x = \sqrt{5 t + 4}$

$y = 4 + 4 / t$

Вариант 23

$x = e^{t} + e^{- t}$

$y = e^{t} - e^{- t}$

Вариант 24

$x = \frac{5 t}{t^{3} + 8}$

$y = \frac{2 t^{2}}{t^{3} + 8}$

Вариант 25

$x = \sqrt{7 t + 7}$

$y = 4 + 3 / t$

Вариант 26

$x = 2 e^{t} + 2 e^{- t}$

$y = 5 e^{t} - 5 e^{- t}$

Вариант 27

$x = \frac{2 t}{t^{3} + 8}$

$y = \frac{4 t^{2}}{t^{3} + 8}$

Вариант 28

$x = \sqrt{3 t + 5}$

$y = 4 + 3 / t$

Вариант 29

$x = e^{t} + e^{- t}$

$y = 7 e^{t} - 7 e^{- t}$

Вариант 30

$x = \frac{2 t}{t^{3} + 8}$

$y = \frac{t^{2}}{t^{3} + 8}$

Вариант 31

$x = \sqrt{4 t + 2}$

$y = 6 + 5 / t$

Вариант 32

$x = 3 e^{t} + 3 e^{- t}$

$y = 2 e^{t} - 2 e^{- t}$

Вариант 33

$x = \frac{5 t}{t^{3} + 8}$

$y = \frac{2 t^{2}}{t^{3} + 8}$

Вариант 34

$x = \sqrt{2 t + 5}$

$y = 5 + 1 / t$

Вариант 35

$x = 5 e^{t} + 5 e^{- t}$

$y = 7 e^{t} - 7 e^{- t}$

Вариант 36

$x = \frac{2 t}{t^{3} + 8}$

$y = \frac{6 t^{2}}{t^{3} + 8}$

Вариант 37

$x = \sqrt{4 t + 3}$

$y = 2 + 7 / t$

Вариант 38

$x = 5 e^{t} + 5 e^{- t}$

$y = 6 e^{t} - 6 e^{- t}$

Вариант 39

$x = \frac{5 t}{t^{3} + 8}$

$y = \frac{2 t^{2}}{t^{3} + 8}$

Вариант 40

$x = \sqrt{4 t + 3}$

$y = 4 + 2 / t$

Вариант 41

$x = 2 e^{t} + 2 e^{- t}$

$y = 5 e^{t} - 5 e^{- t}$

Вариант 42

$x = \frac{6 t}{t^{3} + 27}$

$y = \frac{5 t^{2}}{t^{3} + 27}$

Вариант 43

$x = \sqrt{t + 4}$

$y = 7 + 4 / t$

Вариант 44

$x = 2 e^{t} + 2 e^{- t}$

$y = e^{t} - e^{- t}$

Вариант 45

$x = \frac{7 t}{t^{3} + 27}$

$y = \frac{2 t^{2}}{t^{3} + 27}$

Вариант 46

$x = \sqrt{3 t + 6}$

$y = 5 + 6 / t$

Вариант 47

$x = 5 e^{t} + 5 e^{- t}$

$y = 7 e^{t} - 7 e^{- t}$

Вариант 48

$x = \frac{3 t}{t^{3} + 27}$

$y = \frac{4 t^{2}}{t^{3} + 27}$

Вариант 49

$x = \sqrt{6 t + 2}$

$y = 4 + 5 / t$

Вариант 50

$x = e^{t} + e^{- t}$

$y = 7 e^{t} - 7 e^{- t}$

Вариант 51

$x = \frac{5 t}{t^{3} + 27}$

$y = \frac{7 t^{2}}{t^{3} + 27}$

Вариант 52

$x = \sqrt{2 t + 5}$

$y = 5 + 7 / t$

Вариант 53

$x = e^{t} + e^{- t}$

$y = 2 e^{t} - 2 e^{- t}$

Вариант 54

$x = \frac{2 t}{t^{3} + 8}$

$y = \frac{2 t^{2}}{t^{3} + 8}$

Вариант 55

$x = \sqrt{t + 5}$

$y = 6 + 2 / t$

Вариант 56

$x = e^{t} + e^{- t}$

$y = 3 e^{t} - 3 e^{- t}$

Вариант 57

$x = \frac{7 t}{t^{3} + 8}$

$y = \frac{2 t^{2}}{t^{3} + 8}$

Вариант 58

$x = \sqrt{4 t + 3}$

$y = 1 + 2 / t$

Вариант 59

$x = 2 e^{t} + 2 e^{- t}$

$y = e^{t} - e^{- t}$

Вариант 60

$x = \frac{t}{t^{3} + 27}$

$y = \frac{t^{2}}{t^{3} + 27}$

Вариант 61

$x = \sqrt{5 t + 6}$

$y = 5 + 5 / t$

Вариант 62

$x = 2 e^{t} + 2 e^{- t}$

$y = 7 e^{t} - 7 e^{- t}$

Вариант 63

$x = \frac{7 t}{t^{3} + 27}$

$y = \frac{2 t^{2}}{t^{3} + 27}$

Вариант 64

$x = \sqrt{5 t + 2}$

$y = 5 + 3 / t$

Вариант 65

$x = 2 e^{t} + 2 e^{- t}$

$y = e^{t} - e^{- t}$

Вариант 66

$x = \frac{4 t}{t^{3} + 27}$

$y = \frac{7 t^{2}}{t^{3} + 27}$

Вариант 67

$x = \sqrt{5 t + 4}$

$y = 2 + 1 / t$

Вариант 68

$x = 4 e^{t} + 4 e^{- t}$

$y = 4 e^{t} - 4 e^{- t}$

Вариант 69

$x = \frac{t}{t^{3} + 27}$

$y = \frac{4 t^{2}}{t^{3} + 27}$

Вариант 70

$x = \sqrt{2 t + 6}$

$y = 6 + 6 / t$

Вариант 71

$x = 3 e^{t} + 3 e^{- t}$

$y = 7 e^{t} - 7 e^{- t}$

Вариант 72

$x = \frac{7 t}{t^{3} + 8}$

$y = \frac{2 t^{2}}{t^{3} + 8}$

Вариант 73

$x = \sqrt{t + 5}$

$y = 7 + 5 / t$

Вариант 74

$x = 4 e^{t} + 4 e^{- t}$

$y = e^{t} - e^{- t}$

Вариант 75

$x = \frac{7 t}{t^{3} + 8}$

$y = \frac{5 t^{2}}{t^{3} + 8}$

Вариант 76

$x = \sqrt{5 t + 1}$

$y = 2 + 3 / t$

Вариант 77

$x = 2 e^{t} + 2 e^{- t}$

$y = 2 e^{t} - 2 e^{- t}$

Вариант 78

$x = \frac{6 t}{t^{3} + 8}$

$y = \frac{6 t^{2}}{t^{3} + 8}$

Вариант 79

$x = \sqrt{5 t + 6}$

$y = 4 + 7 / t$

Вариант 80

$x = 6 e^{t} + 6 e^{- t}$

$y = 5 e^{t} - 5 e^{- t}$

Вариант 81

$x = \frac{4 t}{t^{3} + 8}$

$y = \frac{7 t^{2}}{t^{3} + 8}$

Вариант 82

$x = \sqrt{7 t + 6}$

$y = 3 + 5 / t$

Вариант 83

$x = 4 e^{t} + 4 e^{- t}$

$y = 7 e^{t} - 7 e^{- t}$

Вариант 84

$x = \frac{6 t}{t^{3} + 8}$

$y = \frac{4 t^{2}}{t^{3} + 8}$

Вариант 85

$x = \sqrt{7 t + 7}$

$y = 7 + 6 / t$

Вариант 86

$x = 6 e^{t} + 6 e^{- t}$

$y = 7 e^{t} - 7 e^{- t}$

Вариант 87

$x = \frac{2 t}{t^{3} + 27}$

$y = \frac{7 t^{2}}{t^{3} + 27}$

Вариант 88

$x = \sqrt{2 t + 3}$

$y = 6 + 6 / t$

Вариант 89

$x = 2 e^{t} + 2 e^{- t}$

$y = 4 e^{t} - 4 e^{- t}$

Вариант 90

$x = \frac{t}{t^{3} + 27}$

$y = \frac{2 t^{2}}{t^{3} + 27}$

Вариант 91

$x = \sqrt{6 t + 6}$

$y = 2 + 4 / t$

Вариант 92

$x = 6 e^{t} + 6 e^{- t}$

$y = 2 e^{t} - 2 e^{- t}$

Вариант 93

$x = \frac{2 t}{t^{3} + 8}$

$y = \frac{6 t^{2}}{t^{3} + 8}$

Вариант 94

$x = \sqrt{3 t + 4}$

$y = 2 + 1 / t$

Вариант 95

$x = 4 e^{t} + 4 e^{- t}$

$y = 7 e^{t} - 7 e^{- t}$

Вариант 96

$x = \frac{4 t}{t^{3} + 8}$

$y = \frac{2 t^{2}}{t^{3} + 8}$

Вариант 97

$x = \sqrt{5 t + 6}$

$y = 6 + 3 / t$

Вариант 98

$x = 7 e^{t} + 7 e^{- t}$

$y = 6 e^{t} - 6 e^{- t}$

Вариант 99

$x = \frac{5 t}{t^{3} + 27}$

$y = \frac{6 t^{2}}{t^{3} + 27}$

Вариант 100

$x = \sqrt{4 t + 6}$

$y = 4 + 3 / t$

Вариант 101

$x = 2 e^{t} + 2 e^{- t}$

$y = 2 e^{t} - 2 e^{- t}$

Вариант 102

$x = \frac{t}{t^{3} + 8}$

$y = \frac{t^{2}}{t^{3} + 8}$

Вариант 103

$x = \sqrt{6 t + 4}$

$y = 7 + 2 / t$

Вариант 104

$x = e^{t} + e^{- t}$

$y = 5 e^{t} - 5 e^{- t}$

Вариант 105

$x = \frac{7 t}{t^{3} + 27}$

$y = \frac{6 t^{2}}{t^{3} + 27}$

Вариант 106

$x = \sqrt{3 t + 2}$

$y = 6 + 1 / t$

Вариант 107

$x = 4 e^{t} + 4 e^{- t}$

$y = 3 e^{t} - 3 e^{- t}$

Вариант 108

$x = \frac{3 t}{t^{3} + 27}$

$y = \frac{5 t^{2}}{t^{3} + 27}$

Вариант 109

$x = \sqrt{t + 5}$

$y = 4 + 6 / t$

Вариант 110

$x = 4 e^{t} + 4 e^{- t}$

$y = 7 e^{t} - 7 e^{- t}$

Вариант 111

$x = \frac{5 t}{t^{3} + 8}$

$y = \frac{6 t^{2}}{t^{3} + 8}$

Вариант 112

$x = \sqrt{5 t + 2}$

$y = 4 + 2 / t$

Вариант 113

$x = 6 e^{t} + 6 e^{- t}$

$y = e^{t} - e^{- t}$

Вариант 114

$x = \frac{5 t}{t^{3} + 27}$

$y = \frac{3 t^{2}}{t^{3} + 27}$

Вариант 115

$x = \sqrt{5 t + 2}$

$y = 5 + 1 / t$

Вариант 116

$x = 3 e^{t} + 3 e^{- t}$

$y = e^{t} - e^{- t}$

Вариант 117

$x = \frac{t}{t^{3} + 8}$

$y = \frac{t^{2}}{t^{3} + 8}$

Вариант 118

$x = \sqrt{2 t + 4}$

$y = 6 + 2 / t$

Вариант 119

$x = 7 e^{t} + 7 e^{- t}$

$y = 4 e^{t} - 4 e^{- t}$

Вариант 120

$x = \frac{5 t}{t^{3} + 8}$

$y = \frac{7 t^{2}}{t^{3} + 8}$

Вариант 121

$x = \sqrt{4 t + 2}$

$y = 3 + 4 / t$

Вариант 122

$x = 7 e^{t} + 7 e^{- t}$

$y = 2 e^{t} - 2 e^{- t}$

Вариант 123

$x = \frac{6 t}{t^{3} + 8}$

$y = \frac{t^{2}}{t^{3} + 8}$

Вариант 124

$x = \sqrt{6 t + 4}$

$y = 3 + 3 / t$

Вариант 125

$x = 5 e^{t} + 5 e^{- t}$

$y = 5 e^{t} - 5 e^{- t}$

Вариант 126

$x = \frac{2 t}{t^{3} + 8}$

$y = \frac{2 t^{2}}{t^{3} + 8}$

Вариант 127

$x = \sqrt{4 t + 1}$

$y = 2 + 7 / t$

Вариант 128

$x = 5 e^{t} + 5 e^{- t}$

$y = 3 e^{t} - 3 e^{- t}$

Вариант 129

$x = \frac{3 t}{t^{3} + 8}$

$y = \frac{t^{2}}{t^{3} + 8}$

Вариант 130

$x = \sqrt{4 t + 6}$

$y = 7 + 6 / t$

Вариант 131

$x = 2 e^{t} + 2 e^{- t}$

$y = 7 e^{t} - 7 e^{- t}$

Вариант 132

$x = \frac{7 t}{t^{3} + 8}$

$y = \frac{3 t^{2}}{t^{3} + 8}$

Вариант 133

$x = \sqrt{4 t + 1}$

$y = 4 + 3 / t$

Вариант 134

$x = 3 e^{t} + 3 e^{- t}$

$y = 4 e^{t} - 4 e^{- t}$

Вариант 135

$x = \frac{2 t}{t^{3} + 27}$

$y = \frac{t^{2}}{t^{3} + 27}$

Вариант 136

$x = \sqrt{3 t + 3}$

$y = 5 + 6 / t$

Вариант 137

$x = e^{t} + e^{- t}$

$y = 7 e^{t} - 7 e^{- t}$

Вариант 138

$x = \frac{t}{t^{3} + 8}$

$y = \frac{t^{2}}{t^{3} + 8}$

Вариант 139

$x = \sqrt{3 t + 2}$

$y = 7 + 2 / t$

Вариант 140

$x = 6 e^{t} + 6 e^{- t}$

$y = 7 e^{t} - 7 e^{- t}$

Вариант 141

$x = \frac{2 t}{t^{3} + 27}$

$y = \frac{3 t^{2}}{t^{3} + 27}$

Вариант 142

$x = \sqrt{2 t + 5}$

$y = 3 + 2 / t$

Вариант 143

$x = 3 e^{t} + 3 e^{- t}$

$y = e^{t} - e^{- t}$

Вариант 144

$x = \frac{5 t}{t^{3} + 8}$

$y = \frac{5 t^{2}}{t^{3} + 8}$

Вариант 145

$x = \sqrt{5 t + 1}$

$y = 4 + 1 / t$

Вариант 146

$x = 5 e^{t} + 5 e^{- t}$

$y = e^{t} - e^{- t}$

Вариант 147

$x = \frac{4 t}{t^{3} + 8}$

$y = \frac{3 t^{2}}{t^{3} + 8}$

Вариант 148

$x = \sqrt{4 t + 7}$

$y = 6 + 3 / t$

Вариант 149

$x = 5 e^{t} + 5 e^{- t}$

$y = 2 e^{t} - 2 e^{- t}$

Вариант 150

$x = \frac{t}{t^{3} + 27}$

$y = \frac{2 t^{2}}{t^{3} + 27}$



\end{document}